theories/logic/reasoning_os.v
@@ -1,0 +1,93 @@
+
+(* reasoning_os.v *)
+
+From iris.proofmode Require Import base tactics.
+From iris.base_logic.lib Require Import iprop invariants.
+
+(* Hazel Reasoning *)
+From hazel.program_logic Require Import weakest_precondition 
+                                        tactics 
+                                        shallow_handler_reasoning 
+                                        deep_handler_reasoning 
+                                        state_reasoning.
+
+(* Local imports *)
+From haffel.lib Require Import base.
+From haffel.lang Require Import hazel.
+From haffel.lang Require Import subst_map.
+From haffel.logic Require Import iEff.
+From haffel.logic Require Import sem_def.
+From haffel.logic Require Import sem_types.
+From haffel.logic Require Import sem_env.
+From haffel.logic Require Import sem_sub_typing.
+
+
+Section reasoning_os.
+
+  Context `{!heapGS Σ}.
+
+  Definition is_os (σ : sem_sig Σ) : iProp Σ := 
+    ((σ ≤S ⊥) ∨ (∃ τ κ, ⌜ NonExpansive2 τ ⌝ ∗ ⌜ NonExpansive2 κ ⌝ ∗
+                        (σ ≤S (μ∀TS: θ, α, τ θ α ⇒ κ θ α | OS)%S) ∧
+                        ((μ∀TS: θ, α, τ θ α ⇒ κ θ α | OS)%S ≤S σ)))%I.
+
+  Lemma bot_is_os : ⊢ is_os ⊥.
+  Proof. iLeft. iApply sig_le_refl. Qed.
+
+  Lemma os_is_os A B `{ NonExpansive2 A, NonExpansive2 B} : 
+    ⊢ is_os (μ∀TS: θ, α, A θ α ⇒ B θ α | OS)%S.
+  Proof. 
+    iRight. iExists A, B. 
+    do 2 (iSplit; first done).
+    iSplit; iApply sig_le_refl. 
+  Qed.
+
+  Lemma ewp_mono_os σ e Φ Φ' :
+    is_os σ -∗
+    EWP e <| ⊥ |> {| σ |} {{ v, Φ v }} -∗
+    (∀ v : val, Φ v ={⊤}=∗ Φ' v) -∗ EWP e <| ⊥ |> {| σ |} {{ v, Φ' v }}.
+  Proof.
+    iIntros "#HOS Hewp Himp". 
+    iDestruct "HOS" as "[Hbot|(%τ & %κ & (%Hn₁ & %Hn₂ & Hσ₁ & Hσ₂))]".
+    { iApply ewp_ms_prot_mono; [iApply sig_le_nil|].
+      iDestruct (ewp_ms_prot_mono with "Hbot Hewp") as "Hewp'".
+      iApply (ewp_mono with "Hewp' Himp").  }
+    iApply ewp_ms_prot_mono; [iApply "Hσ₂"|].
+    iDestruct (ewp_ms_prot_mono with "Hσ₁ Hewp") as "Hewp".
+    iLöb as "IH" forall (e).
+    rewrite !ewp_unfold /ewp_pre.
+    destruct (to_val e) eqn:?.
+    { iMod "Hewp" as "Hewp". by iApply "Himp". }
+    destruct (to_eff e) eqn:?.
+    - simpl. destruct p eqn:?, p0 eqn:?, m.
+      { iDestruct "Hewp" as "(%Φ'' & [] & ?)". }
+      iDestruct "Hewp" as "(%Φ'' & HΨ & Hps)". 
+      iExists (λ w, Φ'' w ∗ (∀ v, Φ v ={⊤}=∗ Φ' v)%I)%I.
+      iSplitL "HΨ Himp".
+      + rewrite !sem_sig_eff_rec_eq.
+        iDestruct "HΨ" as "(%α & %u & Hrw & HA & HPost)".
+        iExists α, u. iFrame. simpl.
+        iIntros (b) "HB". iFrame. by iApply "HPost".
+      + iDestruct "Hps" as "#Hps".
+        iIntros "!# % (HΦ'' & Himp)". 
+        iSpecialize ("Hps" with "HΦ''"). iNext.
+        iApply ("IH" with "Himp Hps"). 
+    - iIntros (σ₁ ns κ' κs nt) "Hstate".
+      iSpecialize ("Hewp" $! σ₁ ns κ' κs nt with "Hstate"). 
+      iMod "Hewp" as "Hewp". iModIntro.
+      iDestruct "Hewp" as "(Hred & Hpost)".
+      iFrame. iIntros (e₂ σ₂) "Hprim Hcred".
+      iSpecialize ("Hpost" $! e₂ σ₂ with "Hprim Hcred").
+      iInduction (num_laters_per_step) as [|] "IH'"; simpl.
+      { iMod "Hpost" as "Hpost". iModIntro. iNext.
+        do 2 (iMod "Hpost" as "Hpost"; iModIntro).
+        iDestruct "Hpost" as "[$ He₂]".
+        iApply ("IH" with "Himp He₂"). }
+      iMod "Hpost" as "Hpost". iModIntro. iNext.
+      iMod "Hpost" as "Hpost". 
+      iSpecialize ("IH'" with "Himp Hpost").
+      iMod "IH'" as "IH'". do 2 iModIntro. iNext.
+      iApply "IH'".
+  Qed.
+
+End reasoning_os.
